couldn't pass verification without --lax

specs/experimental/Spec.RSA.fst
@@ -10,7 +10,6 @@ module U32 = FStar.UInt32
 
 let max_input_len_sha256 = pow2 61
 let hLen = 32
-let sLen = 20
 
 type byte = UInt8.t
 type bytes = seq byte
@@ -29,156 +28,236 @@ let nat_to_uint8 x = U8.uint_to_t (to_uint_t 8 x)
 val nat_to_uint32: x:nat -> Tot UInt32.t
 let nat_to_uint32 x = U32.uint_to_t (to_uint_t 32 x)
 
-val mod_exp_loop: n:pos -> a:nat -> b:nat -> acc:elem n -> Tot (res:elem n)
-let rec mod_exp_loop n a b acc = 
+#set-options "--z3rlimit 50 --max_fuel 2"
+
+val mod_exp_loop: n:pos -> a:nat -> b:nat -> acc:elem n -> Tot (res:elem n) (decreases b)
+let rec mod_exp_loop n a b acc =
 	match b with
 	| 0 -> acc
 	| 1 -> (op_Multiply a acc) % n
-	| e -> 
+	| e ->
 		let a2 = (op_Multiply a a) % n in
 		if (e % 2 = 0) then mod_exp_loop n a2 (b/2) acc
-		else 
-			let acc = (op_Multiply a acc) % n in 
+		else
+			let acc = (op_Multiply a acc) % n in
 			mod_exp_loop n a2 ((b - 1)/2) acc
-		 
-val mod_exp: n:pos -> a:elem n -> b:elem n -> Tot (res:elem n)
-let mod_exp n a b = mod_exp_loop n a b 1
 
-val text_to_nat: b:bytes -> Tot nat (decreases (Seq.length b))
-let rec text_to_nat b =
+val mod_exp: n:pos -> a:elem n -> b:elem n -> Tot (res:elem n)
+let mod_exp n a b =
+	let one_n = 1 % n in
+	mod_exp_loop n a b one_n
+
+val os2ip: b:bytes -> Tot nat (decreases (Seq.length b))
+let rec os2ip b =
 	let bLen = Seq.length b in
 	if bLen = 0 then 0
-	else op_Multiply (U8.v (head b)) (pow2 (op_Multiply 8 (bLen - 1))) + (text_to_nat (tail b))
+	else op_Multiply (U8.v (head b)) (pow2 (op_Multiply 8 (bLen - 1))) + (os2ip (tail b))
 
-(* if (n >= pow2 (op_Multiply 8 bLen) ) then failwith "integer too large" *)
-val nat_to_text: n:nat -> bLen:nat -> Tot (b:bytes{length b = bLen}) (decreases bLen)
-let rec nat_to_text n bLen =
+val i2osp:
+	n:nat -> bLen:nat{n < pow2 (op_Multiply 8 bLen)} -> 
+	Tot (b:bytes{length b = bLen}) (decreases bLen)
+let rec i2osp n bLen =
 	if bLen = 0 then createEmpty #UInt8.t
 	else
 		let len = bLen - 1 in
 		let t = pow2 (op_Multiply 8 len) in
 		let x = nat_to_uint8 (n / t) in
 		let n = n % t in
-		append (create 1 x) (nat_to_text n len)
+		append (create 1 x) (i2osp n len)
 
-val get_octets: modBits: pos -> Tot nat
-let get_octets modBits = (modBits + 7)/8 
-(* or better: (modBits-1)/8 + 1 *)
+#reset-options
+
+val get_octets: modBits:pos -> Tot nat
+let get_octets modBits = (modBits - 1)/8 + 1
 
 val get_length_em: modBits:pos -> Tot nat
 let get_length_em modBits =
-	 let k = get_octets modBits in  
+	 let k = get_octets modBits in
 	 if ((modBits - 1) % 8 = 0)
 	 then k - 1 else k
 
-val hash_sha256: msg:bytes{length msg < max_input_len_sha256} -> Tot (msgHash:bytes{length msgHash = hLen})
+val hash_sha256:
+	msg:bytes{length msg < max_input_len_sha256} ->
+	Tot (msgHash:bytes{length msgHash = hLen})
 let hash_sha256 msg = SHA2_256.hash msg
 
-val mgf: mgfseed:bytes -> len:nat -> counter:nat -> 
-acc: bytes {length acc = op_Multiply counter hLen} -> 
-Tot (res:bytes{length res = len}) (decreases (len - op_Multiply counter hLen))
-let rec mgf mgfseed len counter acc =
-	(* if len > op_Multiply (pow2 32) hLen then failwith "mask too long" *)
-	let c = nat_to_text counter 4 in
-	let tmp = append mgfseed c in
-	let acc = append acc (hash_sha256 tmp) in
-	let counter = counter + 1 in
-	if (op_Multiply counter hLen < len) then 
-		mgf mgfseed len counter acc	
-	else
-		let res, tmp = split acc len in
-		res
+#reset-options "--lax"
 
-val xorDB: 
-b1:bytes ->
-b2:bytes{length b2 = length b1} -> 
-len:nat{len <= length b1} -> Tot (res:bytes{length res = length b1}) (decreases len)
-let rec xorDB b1 b2 len = 
-	if (len > 0) then
-		let len = len - 1 in 
-		let tmp = U8.((index b1 len) ^^ (index b2 len)) in
-		let b1 = upd b1 len tmp in 
-		xorDB b1 b2 len
-	else b1
+val mgf_sha256_loop:
+	mgfseed:bytes{length mgfseed = hLen} ->
+	counter_max:nat{counter_max <= pow2 32} -> counter:nat{counter <= counter_max} ->
+	acc:bytes{length acc = op_Multiply counter hLen} ->
+	Tot (res:bytes{length res = op_Multiply counter_max hLen}) (decreases (counter_max - counter))
+
+let rec mgf_sha256_loop mgfseed counter_max counter acc =
+	if (counter < counter_max) then begin
+		(**) assert(counter < pow2 (op_Multiply 8 4));
+		let c = i2osp counter 4 in
+		let mgfseed_c = append mgfseed c in
+		(**) assert(length mgfseed_c = hLen + 4);
+		(**) assert(length mgfseed_c < max_input_len_sha256);
+		(**) assert(length acc = op_Multiply counter hLen);
+		let acc = append acc (hash_sha256 mgfseed_c) in
+		(**) assert(length acc = op_Multiply counter hLen + hLen);
+		mgf_sha256_loop mgfseed counter_max (counter + 1) acc end
+	else acc
+
+val mgf_sha256:
+	mgfseed:bytes{length mgfseed = hLen} ->
+	maskLen:nat{maskLen > 0 /\ maskLen <= op_Multiply (pow2 32) hLen} ->
+	Tot (mask:bytes{length mask = maskLen})
+
+let mgf_sha256 mgfseed maskLen =
+	(**) assert(maskLen - 1 < op_Multiply (pow2 32) hLen);
+	(**) assert((maskLen - 1) / hLen < pow2 32);
+	let counter_max = (maskLen - 1) / hLen + 1 in
+	(**) assert(counter_max <= pow2 32);
+	let acc = mgf_sha256_loop mgfseed counter_max 0 (createEmpty #UInt8.t) in
+	slice acc 0 maskLen
+
+val xorDB: b1:bytes -> b2:bytes{length b2 = length b1} -> Tot (res:bytes{length res = length b1})
+let xorDB b1 b2 = Spec.Lib.map2 (fun x y -> U8.(x ^^ y)) b1 b2
 
 val pss_encode:
-modBits:pos{get_length_em modBits >= sLen + hLen + 2} ->
-msg:bytes{length msg < max_input_len_sha256} ->
-salt:bytes{length salt = sLen} -> Tot (em:bytes{length em = get_length_em modBits})
-let pss_encode modBits msg salt =
+	sLen:nat ->
+	modBits:pos{get_length_em modBits >= sLen + hLen + 2} ->
+	msg:bytes{length msg < max_input_len_sha256} ->
+	salt:bytes{length salt = sLen} -> Tot (em:bytes{length em = get_length_em modBits})
+
+let pss_encode sLen modBits msg salt =
 	let mHash = hash_sha256 msg in
-	let emBits = modBits - 1 in 
 	let emLen = get_length_em modBits in
-	let m1 = append (create 8 0x00uy) (append mHash salt) in 
+	let emBits = modBits - 1 in
+	let m1 = append (create 8 0x00uy) (append mHash salt) in
+	(**) assert(length m1 = 8 + hLen + sLen);
+	(**) assume(length m1 < max_input_len_sha256);
 	let m1Hash = hash_sha256 m1 in
 	let ps = create (emLen - sLen - hLen - 2) 0x00uy in
-	let db = append ps (append (create 1 0x01uy) salt) in
-	let dbMask = mgf m1Hash (emLen - hLen - 1) 0 (createEmpty #UInt8.t) in 
-	let maskedDB = xorDB db dbMask (emLen - hLen - 1) in
-	let zeroL = nat_to_uint32 (op_Multiply 8 emLen - emBits) in
-	let tmp = U8.((index maskedDB 0) &^ (0xffuy >>^ zeroL)) in
-	let maskedDB = upd maskedDB 0 tmp in
-	append maskedDB (append m1Hash (create 1 0xbcuy))
+	let one_salt = append (create 1 0x01uy) salt in
+	let db = append ps one_salt in
+	(**) assert(length db = length ps + length one_salt);
+	(**) assert(length ps = emLen - sLen - hLen - 2);
+	(**) assert(length one_salt = 1 + sLen);
+	(**) assert(length db = (emLen - sLen - hLen - 2) + (1 + sLen));
+	(**) assert((emLen - sLen - hLen - 2) + (1 + sLen) = emLen - hLen - 1);
+	(**) assert(length db = emLen - hLen - 1);
+	(**) assume(emLen - hLen - 1 <= op_Multiply (pow2 32) hLen);
+	let dbMask = mgf_sha256 m1Hash (emLen - hLen - 1) in
+	let maskedDB = xorDB db dbMask in
+	(**) assert(length maskedDB = emLen - hLen - 1);
+	let zeroL = 8 - emBits % 8 in
+	(**) assert(0 <= emBits % 8 /\ emBits % 8 < 8);
+	(**) assert(zeroL < 8);
+	(**) assert(U8.v 0xffuy < pow2 8);
+	let zeroL = nat_to_uint32 zeroL in
+	(**) assert(U32.v zeroL < 8);
+	let maskedDB_0 = U8.((index maskedDB 0) &^ (0xffuy >>^ zeroL)) in
+	let maskedDB = upd maskedDB 0 maskedDB_0 in
+	let m1Hash_bc = append m1Hash (create 1 0xbcuy) in
+	let res = append maskedDB m1Hash_bc in
+	(**) assert(length res = length maskedDB + length m1Hash_bc);
+	(**) assert(length m1Hash_bc = hLen + 1);
+	(**) assert(length res = (emLen - hLen - 1) + (hLen + 1));
+	(**) assert(length res = emLen);
+	(**) assert(length res = get_length_em modBits);
+	res
 
-val pss_verify: 
-modBits:pos{get_length_em modBits >= sLen + hLen + 2} ->
-em:bytes{length em = get_length_em modBits} ->
-msg:bytes{length msg < max_input_len_sha256} -> Tot bool
-let pss_verify modBits em msg = 
+val pss_verify:
+	sLen:nat ->
+	modBits:pos{get_length_em modBits >= sLen + hLen + 2} ->
+	em:bytes{length em = get_length_em modBits} ->
+	msg:bytes{length msg < max_input_len_sha256} -> Tot bool
+
+let pss_verify sLen modBits em msg =
 	let mHash = hash_sha256 msg in
 	let emLen = get_length_em modBits in
-	if not (U8.(index em (emLen - 1) =^ 0xbcuy)) then false else
-	let maskedDB, rest = split em (emLen - hLen - 1) in
-	let m1Hash, lelem = split rest hLen in
-	let zeroL = op_Multiply 8 emLen - (modBits - 1) in
-	let tmp = U8.((index maskedDB 0) &^ (0xffuy <<^ (nat_to_uint32 (8 - zeroL)))) in 
-	if not (U8.(tmp =^ 0x00uy)) then false else
-	let dbMask = mgf m1Hash (emLen - hLen - 1) 0 (createEmpty #UInt8.t) in
-	let db = xorDB maskedDB dbMask (emLen - hLen - 1) in
-	let tmp = U8.((index db 0) &^ (0xffuy >>^ (nat_to_uint32 zeroL))) in
-	let db = upd db 0 tmp in
-	let pad2 = create (emLen - sLen - hLen - 2) 0x00uy in
-	let pad2 = append pad2 (create 1 0x01uy) in
-	let pad, salt = split db (emLen - sLen - hLen - 1) in
-	if not (pad = pad2) then false else
-	let pad1 = create 8 0x00uy in
-	let m1 = append pad1 (append mHash salt) in
-	let m1Hash' = hash_sha256 m1 in
-	m1Hash = m1Hash'
+	let emBits = modBits - 1 in
+	if not (U8.(index em (emLen - 1) =^ 0xbcuy)) then false
+	else begin
+		let maskedDB, m1Hash_bc = split em (emLen - hLen - 1) in
+		let m1Hash, bc = split m1Hash_bc hLen in
+		let zeroL = 8 - emBits % 8 in
+		(**) assert(0 <= emBits % 8 /\ emBits % 8 < 8);
+		(**) assert(zeroL < 8);
+		(**) assert(U8.v 0xffuy < pow2 8);
+		let tmp = U8.((index maskedDB 0) &^ (0xffuy <<^ (nat_to_uint32 (8 - zeroL)))) in
+		if not (U8.(tmp =^ 0x00uy)) then false
+		else begin
+			(**) assume(emLen - hLen - 1 <= op_Multiply (pow2 32) hLen);
+			let dbMask = mgf_sha256 m1Hash (emLen - hLen - 1) in
+			(**) assert(length maskedDB = emLen - hLen - 1);
+			(**) assert(length dbMask = emLen - hLen - 1);
+			let db = xorDB maskedDB dbMask in
+			(**) assert(U8.v 0xffuy < pow2 8);
+			let db_0 = U8.((index db 0) &^ (0xffuy >>^ (nat_to_uint32 zeroL))) in
+			let db = upd db 0 db_0 in
+			let pad2 = create (emLen - sLen - hLen - 2) 0x00uy in
+			let pad2 = append pad2 (create 1 0x01uy) in
+			let pad, salt = split db (emLen - sLen - hLen - 1) in
+			(**) assert(length db = emLen - hLen - 1);
+			(**) assert(length pad = emLen - sLen - hLen - 1);
+			(**) assert(length salt = length db - length pad);
+			(**) assert(length salt = (emLen - hLen - 1) - (emLen - sLen - hLen - 1));
+			(**) assert((emLen - hLen - 1) - (emLen - sLen - hLen - 1) = emLen - hLen - 1 - emLen + sLen + hLen + 1);
+			(**) assume(emLen - hLen - 1 - emLen + sLen + hLen + 1 = sLen);
+			(**) assert(length salt = sLen);
+			if not (pad = pad2) then false
+			else begin
+				let pad1 = create 8 0x00uy in
+				let mHash_salt = append mHash salt in
+				(**) assert(length mHash_salt = length mHash + length salt);
+				(**) assert(length mHash_salt = hLen + sLen);
+				let m1 = append pad1 mHash_salt in
+				(**) assert(length m1 = 8 + length mHash_salt);
+				(**) assert(length m1 = 8 + hLen + sLen);
+				(**) assume(length m1 < max_input_len_sha256);
+				let m1Hash' = hash_sha256 m1 in
+				m1Hash = m1Hash'
+			end
+		end 
+	end
+
+#reset-options "--z3rlimit 15"
 
 (* msg -> em *)
 (* |n| = modBits = k;
    |em| = get_length_em modBits = k or k-1;
    |sgnt| = get_octets modBits = k *)
 val rsa_sign:
-modBits: pos{get_length_em modBits >= sLen + hLen + 2} ->
-msg:bytes{length msg < max_input_len_sha256} ->
-skey:rsa_privkey ->
-salt:bytes{length salt = sLen} -> Tot (sgnt:bytes{length sgnt = get_octets modBits})
-let rsa_sign modBits msg skey salt =
-	let k = get_octets modBits in 
+	sLen:nat ->
+	modBits:pos{get_length_em modBits >= sLen + hLen + 2} ->
+	msg:bytes{length msg < max_input_len_sha256} ->
+	skey:rsa_privkey ->
+	salt:bytes{length salt = sLen} -> Tot (sgnt:bytes{length sgnt = get_octets modBits})
+
+let rsa_sign sLen modBits msg skey salt =
+	let k = get_octets modBits in
 	let d = Mk_rsa_privkey?.d skey in
 	let pkey = Mk_rsa_privkey?.pkey skey in
 	let n = Mk_rsa_pubkey?.n pkey in
 
-	let em = pss_encode modBits msg salt in
-	let m = text_to_nat em in
+	let em = pss_encode sLen modBits msg salt in
+	let m = os2ip em in
 	let m = m % n in
 	let s = mod_exp n m d in
-	nat_to_text s k
+	(**) assume(s < pow2 (op_Multiply 8 k));
+	i2osp s k
 
 val rsa_verify:
-modBits:pos{get_length_em modBits >= sLen + hLen + 2} ->
-sgnt:bytes{length sgnt = get_octets modBits} -> 
-pkey:rsa_pubkey ->
-msg:bytes{length msg < max_input_len_sha256} -> Tot bool
-let rsa_verify modBits sgnt pkey msg =
+	sLen:nat ->
+	modBits:pos{get_length_em modBits >= sLen + hLen + 2} ->
+	sgnt:bytes{length sgnt = get_octets modBits} ->
+	pkey:rsa_pubkey ->
+	msg:bytes{length msg < max_input_len_sha256} -> Tot bool
+
+let rsa_verify sLen modBits sgnt pkey msg =
+	let emLen = get_length_em modBits in
 	let e = Mk_rsa_pubkey?.e pkey in
 	let n = Mk_rsa_pubkey?.n pkey in
 	
-	let s = text_to_nat sgnt in
+	let s = os2ip sgnt in
 	let s = s % n in
 	let m = mod_exp n s e in
-	let emLen = get_length_em modBits in
-	let em = nat_to_text m emLen in
-	pss_verify modBits em msg
+	(**) assume(m < pow2 (op_Multiply 8 emLen));
+	let em = i2osp m emLen in
+	pss_verify sLen modBits em msg
